SimpleRef: Add heap operations to big-step semantics

proof/DDC/Language/SimpleRef/Eval.v
@@ -13,17 +13,38 @@ Require Export DDC.Language.SimpleRef.Exp.
     and its final value. 
  *)
 Inductive EVAL : heap -> exp -> heap -> exp -> Prop :=
- | EVDone
+ | EvDone
    :  forall h v2
-   ,  wnfX  v2
+   ,  value  v2
    -> EVAL  h v2 h v2
 
- | EVLamApp
+ | EvLamApp
    :  forall h0 h1 h2 h3 x1 t11 x12 x2 v2 v3
    ,  EVAL h0 x1                h1 (XLam t11 x12)
    -> EVAL h1 x2                h2 v2
    -> EVAL h2 (substX 0 v2 x12) h3 v3
-   -> EVAL h0 (XApp x1 x2)      h3 v3.
+   -> EVAL h0 (XApp x1 x2)      h3 v3
+
+ (* Heap operations *)
+ | EvNewRef
+   :  forall h0 x1 h1 v1
+   ,  EVAL h0 x1      h1 v1         (* evaluate new heap value *)
+   -> EVAL h0        (XNewRef x1)   (* push that value onto the heap *)
+          (v1 <: h1) (XLoc (length h1))
+
+ | EvReadRef
+   :  forall h0 x1 h1 v2 l 
+   ,  EVAL h0 x1 h1 (XLoc l)        (* evaluate heap location *)
+   -> get l h1 = Some v2            (* lookup up that location from the heap *)
+   -> EVAL h0 (XReadRef x1) 
+           h1 v2
+
+ | EvWriteRef
+   :  forall h0 x1 h1 x2 v2 h2 l
+   ,  EVAL h0 x1 h1 (XLoc l)        (* evaluate heap location *)
+   -> EVAL h1 x2 h2 v2              (* evaluate argument to a value *)
+   -> EVAL h0    (XWriteRef x1 x2)  
+           (update l v2 h2) xUnit.  (* update heap with that value*)
 
 Hint Constructors EVAL.
 
@@ -32,44 +53,102 @@ Hint Constructors EVAL.
 Ltac inverts_eval := 
  repeat 
   (match goal with 
-    | [ H: EVAL _ (XApp _ _) _ _ |- _ ] => inverts H
+    | [ H: EVAL _ (XApp _ _)      _ _ |- _ ] => inverts H
+    | [ H: EVAL _ (XNewRef _)     _ _ |- _ ] => inverts H
+    | [ H: EVAL _ (XReadRef _)    _ _ |- _ ] => inverts H
+    | [ H: EVAL _ (XWriteRef _ _) _ _ |- _ ] => inverts H
    end).
 
 
-(* A terminating big-step evaluation always produces a wnf.
+(* Well-formed heaps contain values only. 
+   No free variables or reducible terms in heap cells. *)
+Definition wfH (h: heap) 
+ := Forall value h.
+
+(* A terminating big-step evaluation always produces a wnf, 
+   and preserves the wellformedness of the heap. 
    The fact that the evaluation terminated is implied by the fact
-   that we have a finite proof of EVAL to pass to this lemma. 
- *)
-Lemma eval_produces_wnfX
+   that we have a finite proof of EVAL to pass to this lemma. *)
+Lemma eval_produces_wfH_value
  :  forall h0 x1 h1 v1
- ,  EVAL   h0 x1 h1 v1
- -> wnfX   v1.
+ ,  wfH    h0
+ -> EVAL   h0 x1 h1 v1
+ -> wfH h1 /\ value v1.
 Proof.
- intros. induction H; eauto.
+ intros. induction H0; iauto.
+
+ admit. (* ok, snoc onto heap *)
+
+ eapply Value; burn.
+
+ admit. (* ok, get value from heap *)
+
+ admit. (* ok, update heap, stil wf *)
+
+ unfold xUnit.
+ eapply Value; burn.
 Qed.
-Hint Resolve eval_produces_wnfX.
+
+
+(* A terminating big-step evaluation
+   preserves the wellformedness of the heap *)
+Lemma eval_preserves_wfH
+ :  forall h0 x1 h1 v1
+ ,  wfH h0 
+ -> EVAL h0 x1 h1 v1
+ -> wfH h1.
+Proof.
+ intros.
+ lets D: eval_produces_wfH_value H H0.
+ tauto.
+Qed.
+Hint Resolve eval_preserves_wfH.
+
+
+(* A terminating big-step evaluation
+   produces a value. *)
+Lemma eval_produces_value
+ :  forall h0 x1 h1 v1
+ ,  wfH h0
+ -> EVAL h0 x1 h1 v1
+ -> value v1.
+Proof.
+ intros.
+ lets D: eval_produces_wfH_value H H0.
+ tauto.
+Qed.
+Hint Resolve eval_produces_value.
 
 
 (********************************************************************)
 (** * Big to Small steps *)
-(* Convert a big-step evaluation into a list of individual
+(* Flatten out a big-step evaluation into a list of individual
    machine steps.
+
+   Proof: 
+    This is tedious but straightforward. We assert each of the 
+    intermediate STEPS to get the intermediate values, then use
+    preservation to show the results have the same type as before.
+    Once we've got a STEPS for each of the hyps of the EVAL we're
+    we're flattening, join them all together with an EsAppend,
+    stating the contexts we're performing the reductions in.
  *)
 Lemma steps_of_eval
  :  forall se h0 h1 x1 t1 x2
- ,  TYPEH se  h0
+ ,  wfH h0 -> TYPEH se  h0
  -> TYPE  nil se x1 t1
  -> EVAL  h0  x1 h1 x2
  -> STEPS h0  x1 h1 x2.
 Proof.
- intros se h0 h1 x1 t1 v2 HTH HT HE. gen se t1.
+ intros se h0 h1 x1 t1 v2 HTW HTH HT HE. gen se t1.
 
  (* Induction over the form of (EVAL x1 x2) *)
  induction HE; intros.
- Case "EVDone".
+ Case "EvDone".
   apply EsNone.
 
- Case "EVLamApp".
+ (* Function Application **********)
+ Case "EvLamApp".
   inverts_type. 
    rename H3 into Tx1.
    rename H5 into Tx2.
@@ -79,7 +158,7 @@ Proof.
    eauto. clear IHHE1.
   lets Rx1: preservation_steps HTH Tx1 Sx1.
    destruct Rx1 as [se1]. int.
-   inverts_type. 
+   inverts keep H2.
 
   (* evaluate arg *)
   assert (TYPE  nil se1 x2 t0). iauto.
@@ -87,7 +166,7 @@ Proof.
    iauto. clear IHHE2.
   lets Rx1: preservation_steps se1 h1 x2 t0 h2.
   lets Rx1': Rx1 v2. clear Rx1. int.
-  destruct H2 as [se2]. int.
+  destruct H3 as [se2]. int.
 
   (* perform substitution *)
   assert (TYPE  nil se2 (substX 0 v2 x12) t1).
@@ -95,19 +174,80 @@ Proof.
   assert (STEPS h2 (substX 0 v2 x12) h3 v3). eauto.
   lets Rx2: preservation_steps se2 h2 (substX 0 v2 x12) t1 h3.
   lets Rx2': Rx2 v3. clear Rx2. int.
-  destruct H8 as [se3]. int.
+  destruct H9 as [se3]. int.
 
   eapply EsAppend.
     lets D: steps_context XcApp1.
      eapply D. eauto.
   eapply EsAppend.
    lets D: steps_context XcApp2.
-    assert (wnfX (XLam t0 x12)) as WL. auto. eapply WL.
-    eapply D. eauto.
+    assert (wnfX (XLam t0 x12)) as WL. auto.
+     assert (closedX (XLam t0 x12)). 
+     eauto. eauto. eapply D. eauto.
+
   eapply EsAppend.
    eapply EsStep.
     eapply EsLamApp. eauto.
     eauto.
+
+
+ (* Create a new Reference *******)
+ Case "EvNewRef".
+  inverts_type.
+   rename H2 into Tx1.
+  
+  (* evaluate argument *)
+  assert (STEPS h0 x1 h1 v1) as Sx1.
+   eauto. clear IHHE.
+  lets Rx1: preservation_steps HTH Tx1 Sx1.
+   destruct Rx1 as [se1]. int.
+  
+  eapply EsAppend.
+   lets D: steps_context XcNewRef.
+    eapply D. eauto.
+  eapply EsStep. eauto.
+
+
+ (* Read a reference ************)
+ Case "EvReadRef".
+  inverts_type.
+   rename H3 into Tx1.
+  
+  (* evaluate argument to a location *)  
+  assert (STEPS h0 x1 h1 (XLoc l)) as Sx1.
+   eauto. clear IHHE.
+  lets Rx1: preservation_steps HTH Tx1 Sx1.
+   destruct Rx1 as [se1]. int.
+ 
+  eapply EsAppend.
+   lets D: steps_context XcReadRef.
+    eapply D. eauto.
+  eapply EsStep. eauto.
+
+
+ (* Write a reference **********)
+ Case "EvWriteRef".
+  inverts_type.
+   rename H3 into Tx1.
+   rename H5 into Tx2.
+
+  (* evaluate first argument to a location *)
+  assert (STEPS h0 x1 h1 (XLoc l)) as Sx1.
+   eauto. clear IHHE1.
+  lets Rx1: preservation_steps HTH Tx1 Sx1.
+   destruct Rx1 as [se1]. int.
+
+  (* evaluate second argument to a value *)
+  assert (STEPS h1 x2 h2 v2) as Sx2.
+   eauto. clear IHHE2.
+  assert (TYPE nil se1 x2 tData) as Tx2'. 
+   eauto.
+  lets Rx2: preservation_steps H Tx2' Sx2.
+   destruct Rx2 as [se2]. int.
+
+  eapply EsAppend.
+   lets D: steps_context XcWriteRef1. eapply D. eauto.
+   lets D: steps_context XcWriteRef2; eauto.
 Qed.
 
 
@@ -124,37 +264,25 @@ Qed.
  *)
 (*
 Lemma eval_expansion
- :  forall te x1 t1 x2 v3
- ,  TYPE te x1 t1
- -> STEP x1 x2 -> EVAL x2 v3 
- -> EVAL x1 v3.
+ :  forall se te h1 x1 t1 h2 x2 h3 v3
+ ,  TYPE se te x1 t1
+ -> STEP h1 x1  h2 x2 -> EVAL h2 x2  h3 v3 
+ -> EVAL h1 x1  h3 v3.
 Proof.
- intros. gen te t1 v3.
+ intros. gen se te t1 h3 v3.
 
  (* Induction over the form of (STEP x1 x2) *)
  induction H0; intros.
 
  Case "eval in context".
-  destruct H. 
 
-  SCase "top level".
-   eauto.
- 
-  SCase "x1 steps".
-   inverts H1. inverts H2.
-    inverts H.
-    eapply EVLamApp; eauto.
 
-  SCase "x2 steps".
-   inverts H1. inverts H2.
-   inverts H1.
+
+  SCase "XApp".
    eapply EVLamApp; eauto.
 
-  SCase "application".
-   eapply EVLamApp.
-    eauto.
-    inverts H. 
-    apply EVDone. auto. auto.
+  SCase "XNewRef".
+   eapply EV
 Qed.
 
 
